\documentclass[a4paper]{article}
\usepackage{setspace}
\usepackage[T2A]{fontenc} %
\usepackage[utf8]{inputenc} % подключение русского языка
\usepackage[russian]{babel} %
\usepackage[14pt]{extsizes}
\usepackage{mathtools}
\usepackage{graphicx}
\usepackage{fancyhdr}
\usepackage{amssymb}
\usepackage{amsmath, amsfonts, amssymb, amsthm, mathtools}
\usepackage{tikz}

\usetikzlibrary{positioning}
\setstretch{1.3}

\newcommand{\mat}[1]{\begin{pmatrix} #1 \end{pmatrix}}
\renewcommand{\f}[2]{\frac{#1}{#2}}
\newcommand{\dspace}{\space\space}
\newcommand{\s}[2]{\sum\limits_{#1}^{#2}}
\newcommand{\sq}[1]{\left[ {#1} \right]}
\newcommand{\gath}[1]{\left[ \begin{array}{@{}l@{}} #1 \end{array} \right.}
\newcommand{\case}[1]{\begin{cases} #1 \end{cases}}
\newcommand{\ts}{\text{\space}}

\newcommand{\lr}{\Leftrightarrow}
\renewcommand{\r}{\Rightarrow}
\newcommand{\rr}{\rightarrow}
\renewcommand{\geq}{\geqslant}
\renewcommand{\leq}{\leqslant}
\newcommand{\RR}{\mathbb{R}}
\newcommand{\CC}{\mathbb{C}}
\newcommand{\QQ}{\mathbb{Q}}
\newcommand{\ZZ}{\mathbb{Z}}
\newcommand{\VV}{\mathbb{V}}
\newcommand{\NN}{\mathbb{N}}

\DeclarePairedDelimiter\abs{\lvert}{\rvert} %
\makeatletter                               % \abs{}
\let\oldabs\abs                             %
\def\abs{\@ifstar{\oldabs}{\oldabs*}}       %

\begin{document}

\section*{Домашнее задание на 2.10.2024 (Линейная алгебра)}
{\large Емельянов Владимир, ПМИ гр №247}\\\\
\begin{enumerate}
    \item[\textbf{1.}]
    \begin{enumerate}
        \item[1.1.]
        $$X\cdot \mat{3 & -2 \\ 5 & -4} = \mat{-1 & 2 \\ -5 & 6}$$
        $$\mat{3 & 5 \\ -2 & -4} \cdot X^T = \mat{-1 & -5 \\ 2 & 6}$$
        $$A = \mat{3 & 5 & | & -1 & -5\\ -2 & -4 & | & 2 & 6}$$
        $$A[0] = A[0]/3$$
        $$\mat{1 & \f{5}{3} & | & \f{-1}{3} & \f{-5}{3}\\ -2 & -4 & | & 2 & 6}$$
        $$A[1] = A[1]+2A[0]$$
        $$\mat{1 & \f{5}{3} & | & \f{-1}{3} & \f{-5}{3}\\ 0 & -\f{2}{3} & | & \f{4}{3} & \f{8}{3}}$$
        $$A[1] = A[1]\cdot \f{-3}{2}$$
        $$\mat{1 & \f{5}{3} & | & \f{-1}{3} & \f{-5}{3}\\ 0 & 1 & | & -2 & -4}$$
        $$A[0] = A[0]-A[1]\cdot \f{5}{3}$$
        $$\mat{1 & 0 & | & 3 & 5\\ 0 & 1 & | & -2 & -4}$$
        $$\case{
            x_1 = 3\\
            x_2 = -2\\
            y_1 = 5 \\
            y_2 = -4 
        }\r X^T = \mat{3 & 5 \\ -2 & -4} \r X = \mat{3 & -2 \\ 5 & -4}$$ 

        \item[1.2.]
        $$\mat{3 & -1 \\ 5 & -2} X \mat{5 & 6 \\ 7 & 8} = \mat{14 & 16 \\ 9 & 10}$$
        $$Y = X \mat{5 & 6 \\ 7 & 8}$$
        $$\mat{3 & -1 \\ 5 & -2} Y = \mat{14 & 16 \\ 9 & 10}$$
        $$A = \mat{3 & -1 & | & 14 & 16\\ 5 & -2 & | & 9 & 10}$$
        $$A[0] = A[0]/3$$
        $$\mat{1 & -\f{1}{3} & | & \f{14}{3} & \f{16}{3}\\ 5 & -2 & | & 9 & 10}$$
        $$A[1] = A[1]- 5A[0]$$
        $$\mat{1 & -\f{1}{3} & | & \f{14}{3} & \f{16}{3}\\ 0 & -\f{1}{3} & | & -\f{43}{3} & -\f{50}{3}}$$
        $$A[0] = A[0]-A[1]$$
        $$\mat{1 & 0 & | & 19 & 22\\ 0 & -\f{1}{3} & | & -\f{43}{3} & -\f{50}{3}}$$
        $$A[1] = A[1]\cdot(-3)$$
        $$\mat{1 & 0 & | & 19 & 22\\ 0 & 1 & | & 43 & 50} \r Y = \mat{19 & 22 \\ 43 & 50} = X \mat{5 & 6 \\ 7 & 8}$$
        $$\mat{5 & 7 \\ 6 & 8}X^T = \mat{19 & 43 \\ 22 & 50}$$
        $$\mat{5 & 7 & | & 19 & 43\\ 6 & 8 & | & 22 & 50}$$
        $$A[0] = A[0]/5$$
        $$\mat{1 & \f{7}{5} & | & \f{19}{5} & \f{43}{5}\\ 6 & 8 & | & 22 & 50}$$
        $$A[1] = A[1]-6A[0]$$
        $$\mat{1 & \f{7}{5} & | & \f{19}{5} & \f{43}{5} \\ 0 & -\f{2}{5} & | & -\f{4}{5} & -\f{8}{5}}$$
        $$A[1] = -5*A[1]/2$$
        $$\mat{1 & \f{7}{5} & | & \f{19}{5} & \f{43}{5} \\ 0 & 1 & | & 2 & 4}$$
        $$A[0] = A[0]-7*A[1]/5$$
        $$\mat{1 & 0 & | & 1 & 3 \\ 0 & 1 & | & 2 & 4} \r X^T = \mat{1 & 3 \\ 2 & 4} \r X = \mat{1 & 2 \\ 3 & 4}$$
    
        \item[1.3]
        $$\mat{3 & -1 & 2 \\ 4 & -3 & 3 \\ 1 & 3 & 0}X = \mat{3 & 7 \\ 1 & 7 \\ 7 & 7}$$
        $$A = \mat{3 & -1 & 2 & | & 3 & 7\\ 4 & -3 & 3 & | & 1 & 7 \\ 1 & 3 & 0 & | & 7 & 7}$$
        $$A[0] = A[0]/3$$
        $$\mat{1 & -\f{1}{3} & \f{2}{3} & | & 1 & \f{7}{3} \\ 4 & -3 & 3 & | & 1 & 7 \\ 1 & 3 & 0 & | & 7 & 7}$$
        $$A[1] = A[1]-4*A[0]$$
        $$\mat{1 & -\f{1}{3} & \f{2}{3} & | & 1 & \f{7}{3} \\ 0 & -\f{5}{3} & \f{1}{3} & | & -3 & -\f{7}{3} \\ 1 & 3 & 0 & | & 7 & 7}$$
        $$A[1] = A[1]*(-3)/5$$
        $$\mat{1 & -\f{1}{3} & \f{2}{3} & | & 1 & \f{7}{3} \\ 0 & 1 & -\f{1}{5} & | & \f{9}{5} & \f{7}{5} \\ 1 & 3 & 0 & | & 7 & 7}$$
        $$A[2] = A[2]-A[0]$$
        $$\mat{1 & -\f{1}{3} & \f{2}{3} & | & 1 & \f{7}{3} \\ 0 & 1 & -\f{1}{5} & | & \f{9}{5} & \f{7}{5} \\ 0 & \f{10}{3} & -\f{2}{3} & | & 6 & \f{14}{3}}$$
        $$A[2] = A[2]*3/10$$
        $$\mat{1 & -\f{1}{3} & \f{2}{3} & | & 1 & \f{7}{3} \\ 0 & 1 & -\f{1}{5} & | & \f{9}{5} & \f{7}{5} \\ 0 & 1 & -\f{1}{5} & | & \f{9}{5} & \f{7}{5}} = \mat{1 & -\f{1}{3} & \f{2}{3} & | & 1 & \f{7}{3} \\ 0 & 1 & -\f{1}{5} & | & \f{9}{5} & \f{7}{5}}$$
        $$A[0] = A[0]+A[1]/3$$
        $$\mat{1 & 0 & \f{3}{5} & | & \f{8}{5} & \f{14}{5} \\ 0 & 1 & -\f{1}{5} & | & \f{9}{5} & \f{7}{5}}$$
        $$\case{
            x_1 +\f{3}{5}x_3 = \f{8}{5}\\
            x_2 -\f{1}{5}x_3 = \f{9}{5}\\
            y_1 +\f{3}{5}y_3 = \f{14}{5}\\
            y_2 -\f{1}{5}y_3 = \f{7}{5}
        } \r X = \mat{\f{8}{5}-\f{3}{5}x_3 & \f{14}{5}-\f{3}{5}y_3 \\ \f{9}{5}+\f{1}{5}x_3 & \f{7}{5}+\f{1}{5}y_3 \\ x_3 & y_3} , \forall x_3, y_3 \in \RR$$
        
        \item[1.4]
        $$A^TX+X =B, \text{\space} A = \mat{0 & 2 \\ -1 & -3}, B = \mat{2 & 0 & 3 \\ 4 & 0 & 6}$$
        $$(A^T+E)X = B$$
        $$(\mat{0 & -1 \\ 2 & -3}+E)X=\mat{2 & 0 & 3 \\ 4 & 0 & 6}$$
        $$\mat{1 & -1 \\ 2 & -2}X=\mat{2 & 0 & 3 \\ 4 & 0 & 6}$$
        $$C = \mat{1 & -1 & | & 2 & 0 & 3 \\ 2 & -2 & | & 4 & 0 & 6}$$
        $$C[1] = C[1]-2*C[0]$$
        $$\mat{1 & -1 & | & 2 & 0 & 3 \\ 0 & 0 & | & 0 & 0 & 0} = \mat{1 & -1 & | & 2 & 0 & 3}$$
        $$\case{
            x_1 -x_2 = 2\\
            y_1 -y_2 = 0\\
            z_1 -z_2 = 3
        }\r X = \mat{2+x_2 & y_2 & 3+z_2 \\ x_2 & y_2 & z_2} \ts \forall x_2,y_2,z_2 \in \RR$$
        
    \end{enumerate}

    \item[\textbf{2.}]
    $$\mat{
    1 & 1 & 1 & \ldots & 1 \\
    0 & 1 & 1 & \ldots & 1 \\
    0 & 0 & 1 & \ldots & 1 \\
    \vdots & \ddots & \ddots & \ddots & \vdots \\
    0 & 0 & \ldots & 0 & 1}X 
    = \mat{
    1 & 2 & 3 & \ldots & n \\
    0 & 1 & 2 & \ldots & n-1 \\
    0 & 0 & 1 & \ddots & n-2 \\
    \vdots & \ddots & \ddots & \ddots & \vdots \\
    0 & 0 & \ldots & 0 & 1
    }$$
    $$A = \mat{
    1 & 1 & 1 & \ldots & 1  & 1 & 2 & 3 & \ldots & n\\
    0 & 1 & 1 & \ldots & 1  & 0 & 1 & 2 & \ldots & n-1\\
    0 & 0 & 1 & \ldots & 1  & 0 & 0 & 1 & \ddots & n-2\\
    \vdots & \ddots & \ddots & \ddots & \vdots  & \vdots & \ddots & \ddots & \ddots & \vdots\\
    0 & 0 & \ldots & 0 & 1 & 0 & 0 & \ldots & 0 & 1 }$$
    $$A[0] = A[0] - A[1]$$
    $$A[1] = A[1] - A[2]$$
    $$\dots$$
    $$A[n-1] = A[n-1]-A[n]$$

    $$\mat{
    1 & 0 & 0 & \ldots & 0  & 1 & 1 & 1 & \ldots & 1\\
    0 & 1 & 0 & \ldots & 0  & 0 & 1 & 1 & \ldots & 1\\
    0 & 0 & 1 & \ldots & 0  & 0 & 0 & 1 & \ddots & 1\\
    \vdots & \ddots & \ddots & \ddots & \vdots  & \vdots & \ddots & \ddots & \ddots & \vdots\\
    0 & 0 & \ldots & 0 & 1 & 0 & 0 & \ldots & 0 & 1 } \r X=\mat{
    1 & 1 & 1 & \ldots & 1 \\
    0 & 1 & 1 & \ldots & 1 \\
    0 & 0 & 1 & \ldots & 1 \\
    \vdots & \ddots & \ddots & \ddots & \vdots \\
    0 & 0 & \ldots & 0 & 1}$$
    \textbf{Ответ: } $X=\mat{
        1 & 1 & 1 & \ldots & 1 \\
        0 & 1 & 1 & \ldots & 1 \\
        0 & 0 & 1 & \ldots & 1 \\
        \vdots & \ddots & \ddots & \ddots & \vdots \\
        0 & 0 & \ldots & 0 & 1}$
    \item[\textbf{3.}]
    \begin{enumerate}
        \item[3.1.]
        $A = \mat{1 & 2 \\ 4 & 5} \ts A^{-1} - ?$\\
        $$\mat{1 & 2 \\ 4 & 5}A^{-1} = \mat{1 & 0\\ 0 & 1}$$
        $$C = \mat{1 & 2 & | & 1 & 0\\ 4 & 5 & | & 0 & 1}$$
        $$C[1] = C[1]-4C[0]$$
        $$\mat{1 & 2 & | & 1 & 0\\ 0 & -3 & | & -4 & 1}$$
        $$C[1] = C[1]/-3$$
        $$\mat{1 & 2 & | & 1 & 0 \\ 0 & 1 & | & \f{4}{3} & -\f{1}{3}}$$
        $$C[0] = C[0]-2*C[1]$$
        $$\mat{1 & 0 & | & -\f{5}{3} & \f{2}{3} \\ 0 & 1 & | & \f{4}{3} & -\f{1}{3}}\r A^{-1} = \mat{-\f{5}{3} & \f{2}{3} \\ \f{4}{3} & -\f{1}{3}}$$
        \textbf{Ответ: } $A^{-1} = \mat{-\f{5}{3} & \f{2}{3} \\ \f{4}{3} & -\f{1}{3}}$

        \item[3.2.]
        $A = \mat{1 & 2 & 3 \\ 4 & 5 & 6 \\ 7 & 8 & 9 } \ts A^{-1}-?$
        $$\mat{1 & 2 & 3 \\ 4 & 5 & 6 \\ 7 & 8 & 9 }A^{-1}=\mat{1 & 0 & 0 \\ 0 & 1 & 0 \\ 0 & 0 & 1}$$
        $$C = \mat{1 & 2 & 3 & | & 1 & 0 & 0 \\ 4 & 5 & 6 & | & 0 & 1 & 0 \\ 7 & 8 & 9 & | & 0 & 0 & 1}$$
        $$C[1] = C[1]-4*C[0]$$
        $$\mat{1 & 2 & 3 & | & 1 & 0 & 0 \\ 0 & -3 & -6 & | & -4 & 1 & 0 \\ 7 & 8 & 9 & | & 0 & 0 & 1}$$
        $$C[1] = C[1]/-3$$
        $$\mat{1 & 2 & 3 & | & 1 & 0 & 0 \\ 0 & 1 & 2 & | & \f{4}{3} & -\f{1}{3} & 0 \\ 7 & 8 & 9 & | & 0 & 0 & 1}$$
        $$C[2] = C[2] - 7*C[0]$$
        $$\mat{1 & 2 & 3 & | & 1 & 0 & 0 \\ 0 & 1 & 2 & | & \f{4}{3} & -\f{1}{3} & 0 \\ 0 & -6 & -12 & | & -7 & 0 & 1}$$
        $$C[2] = C[2] + 6*C[1]$$
        $$\mat{1 & 2 & 3 & | & 1 & 0 & 0 \\ 0 & 1 & 2 & | & \f{4}{3} & -\f{1}{3} & 0 \\ 0 & 0 & 0 & | & 1 & -2 & 1}$$
        $$0 = 1 \text{ - } \varnothing$$
        \textbf{Ответ: } нет

        \item[3.3.]
        $A = \mat{2 & 7 & 3 \\ 3 & 9 & 4 \\ 1 & 5 & 3} \ts A^{-1} - ?$
        $$\mat{2 & 7 & 3 \\ 3 & 9 & 4 \\ 1 & 5 & 3}A^{-1} = \mat{1 & 0 & 0\\ 0 & 1 & 0 \\ 0 & 0 & 1}$$
        $$C = \mat{2 & 7 & 3 & | & 1 & 0 & 0\\ 3 & 9 & 4 & | & 0 & 1 & 0 \\ 1 & 5 & 3 & | & 0 & 0 & 1}$$
        $$C[0] = C[0]/2$$
        $$\mat{1 & \f{7}{2} & \f{3}{2} & | & \f{1}{2} & 0 & 0 \\ 3 & 9 & 4 & | & 0 & 1 & 0 \\ 1 & 5 & 3 & | & 0 & 0 & 1}$$
        $$C[1] = C[1] - 3*C[0]$$
        $$\mat{1 & \f{7}{2} & \f{3}{2} & | & \f{1}{2} & 0 & 0 \\ 0 & -\f{3}{2} & -\f{1}{2} & | & -\f{3}{2} & 1 & 0 \\ 1 & 5 & 3 & | & 0 & 0 & 1}$$
        $$C[1] = C[1]*-2/3$$
        $$\mat{1 & \f{7}{2} & \f{3}{2} & | & \f{1}{2} & 0 & 0 \\ 0 & 1 & \f{1}{3} & | & 1 & -\f{2}{3} & 0 \\ 1 & 5 & 3 & | & 0 & 0 & 1}$$
        $$C[2] = C[2] - C[0]$$
        $$\mat{1 & \f{7}{2} & \f{3}{2} & | & \f{1}{2} & 0 & 0 \\ 0 & 1 & \f{1}{3} & | & 1 & -\f{2}{3} & 0 \\ 0 & \f{3}{2} & \f{3}{2} & | & -\f{1}{2} & 0 & 1}$$
        $$C[2] = C[2]-C[1]*3/2$$
        $$\mat{1 & \f{7}{2} & \f{3}{2} & | & \f{1}{2} & 0 & 0 \\ 0 & 1 & \f{1}{3} & | & 1 & -\f{2}{3} & 0 \\ 0 & 0 & 1 & | & -2 & 1 & 1}$$
        $$C[0] = C[0] - C[1]*7/2$$
        $$\mat{1 & 0 & \f{1}{3} & | & -3 & \f{7}{3} & 0 \\ 0 & 1 & \f{1}{3} & | & 1 & -\f{2}{3} & 0 \\ 0 & 0 & 1 & | & -2 & 1 & 1}$$
        $$C[0] = C[0] - C[2]/3$$
        $$\mat{1 & 0 & 0 & | & -\f{7}{3} & 2 & -\f{1}{3} \\ 0 & 1 & \f{1}{3} & | & 1 & -\f{2}{3} & 0 \\ 0 & 0 & 1 & | & -2 & 1 & 1}$$
        $$C[1] = C[1] - C[2]/3$$
        $$\mat{1 & 0 & 0 & | & -\f{7}{3} & 2 & -\f{1}{3} \\ 0 & 1 & 0 & | & \f{5}{3} & -1 & -\f{1}{3} \\ 0 & 0 & 1 & | & -2 & 1 & 1} \r A^{-1}= \mat{-\f{7}{3} & 2 & -\f{1}{3} \\ \f{5}{3} & -1 & -\f{1}{3} \\ -2 & 1 & 1}$$
        \textbf{Ответ: } $A^{-1}= \mat{-\f{7}{3} & 2 & -\f{1}{3} \\ \f{5}{3} & -1 & -\f{1}{3} \\ -2 & 1 & 1}$
    \end{enumerate}

    \item[\textbf{4.}]
    $$C = (A|E) = \mat{2 & 10 & 3 & | & 1 & 0 \\ 1 & 5 & 4 & | & 0 & 1}$$
    $$C[0], C[1] = C[1], C[0]$$
    $$\mat{ 1 & 5 & 4 & | & 0 & 1 \\ 2 & 10 & 3 & | & 1 & 0}$$
    $$C[1] = C[1] - 2*C[0]$$
    $$\mat{1 & 5 & 4 & | & 0 & 1 \\ 0 & 0 & -5 & | & 1 & -2}$$
    $$C[1] = C[1]/-5$$
    $$\mat{1 & 5 & 4 & | & 0 & 1 \\ 0 & 0 & 1 & | & -\f{1}{5} & \f{2}{5}}$$
    $$C[0] = C[0] - 4*C[1]$$
    $$(A'|U) = \mat{1 & 5 & 0 & | & \f{4}{5} & -\f{3}{5} \\ 0 & 0 & 1 & | & -\f{1}{5} & \f{2}{5}} \r U = \mat{\f{4}{5} & -\f{3}{5} \\ -\f{1}{5} & \f{2}{5}}$$
    $$UA = \mat{\f{4}{5} & -\f{3}{5} \\ -\f{1}{5} & \f{2}{5}} \cdot \mat{2 & 10 & 3 \\ 1 & 5 & 4} = \mat{1 & 5 & 0 \\ 0 & 0 & 1} = A' \text{ - верно}$$
    \textbf{Ответ:} $U = \mat{\f{4}{5} & -\f{3}{5} \\ -\f{1}{5} & \f{2}{5}}$

    \item[\textbf{5.}]
    $$A = \mat{0 & 1 & 1 & \dots & 1 \\
           1 & 0 & 1 & \dots & 1 \\
           \dots & \dots & \dots & \dots & \dots \\
           1 & 1 & 1 & \dots & 0}$$
    $$A\cdot A^{-1} = E$$
    $$(A|E) = C = \mat{0 & 1 & 1 & \dots & 1 & 1 & 0 & 0 & \dots & 0\\
                       1 & 0 & 1 & \dots & 1 & 0 & 1 & 0 & \dots & 0\\
                       \dots & \dots & \dots & \dots & \dots & \dots & \dots & \dots & \dots & \dots\\
                       1 & 1 & 1 & \dots & 0 & 0 & 0 & 0 & \dots & 1}$$

    $$C[1, 2, 3 \dots, n] = C[1, 2, 3, \dots, n]-C[0]$$
    $$\mat{0 & 1 & 1 & \dots & 1 & 1 & 0 & 0 & \dots & 0\\
            1 & -1 & 0 & \dots & 0 & -1 & 1 & 0 & \dots & 0\\
            \dots & \dots & \dots & \dots & \dots & \dots & \dots & \dots & \dots & \dots\\
            1 & 0 & 0 & \dots & -1 & -1 & 0 & 0 & \dots & 1}$$
    $$C[0] = C[1, 2, 3, \dots, n] + C[0]$$
    $$\mat{n-1 & 0 & 0 & \dots & 0 & 2-n & 1 & 1 & \dots & 1\\
            1 & -1 & 0 & \dots & 0 & -1 & 1 & 0 & \dots & 0\\
            \dots & \dots & \dots & \dots & \dots & \dots & \dots & \dots & \dots & \dots\\
            1 & 0 & 0 & \dots & -1 & -1 & 0 & 0 & \dots & 1}$$
    $$C[0] = C[0]/(n-1)$$
    $$\mat{1 & 0 & 0 & \dots & 0 & \f{2-n}{n-1} & \f{1}{n-1} & \f{1}{n-1} & \dots & \f{1}{n-1}\\
            1 & -1 & 0 & \dots & 0 & -1 & 1 & 0 & \dots & 0\\
            \dots & \dots & \dots & \dots & \dots & \dots & \dots & \dots & \dots & \dots\\
            1 & 0 & 0 & \dots & -1 & -1 & 0 & 0 & \dots & 1}$$
    $$C[1, 2, 3, \dots, n] =C[1, 2, 3, \dots, n] - C[0] $$
    $$\mat{1 & 0 & 0 & \dots & 0 & \f{2-n}{n-1} & \f{1}{n-1} & \f{1}{n-1} & \dots & \f{1}{n-1}\\
            0 & -1 & 0 & \dots & 0 & -1 - \f{2-n}{n-1} & 1 - \f{1}{n-1} & -\f{1}{n-1} & \dots & -\f{1}{n-1}\\
            \dots & \dots & \dots & \dots & \dots & \dots & \dots & \dots & \dots & \dots\\
            0 & 0 & 0 & \dots & -1 & -1 - \f{2-n}{n-1} & -\f{1}{n-1} & -\f{1}{n-1} & \dots & 1-\f{1}{n-1}}$$
    $$C[1, 2, 3, \dots, n] = -C[1, 2, 3, \dots, n]$$
    $$\mat{1 & 0 & 0 & \dots & 0 & \f{2-n}{n-1} & \f{1}{n-1} & \f{1}{n-1} & \dots & \f{1}{n-1}\\
            0 & 1 & 0 & \dots & 0 & 1 + \f{2-n}{n-1} & \f{1}{n-1}-1 & \f{1}{n-1} & \dots & \f{1}{n-1}\\
            \dots & \dots & \dots & \dots & \dots & \dots & \dots & \dots & \dots & \dots\\
            0 & 0 & 0 & \dots & 1 & 1 + \f{2-n}{n-1} & \f{1}{n-1} & \f{1}{n-1} & \dots & \f{1}{n-1}-1} \r$$
    $$A^{-1} = \mat{\f{2-n}{n-1} & \f{1}{n-1} & \f{1}{n-1} & \dots & \f{1}{n-1} \\
                    1 + \f{2-n}{n-1} & \f{1}{n-1}-1 & \f{1}{n-1} & \dots & \f{1}{n-1}\\
                    \dots & \dots & \dots & \dots & \dots\\
                    1 + \f{2-n}{n-1} & \f{1}{n-1} & \f{1}{n-1} & \dots & \f{1}{n-1}-1}$$

\end{enumerate}

\end{document}